Finished XArea

XArea.v
@@ -1,25 +1,27 @@
 From Elo Require Import Core.
 From Elo Require Import Properties1.
 
+From Elo Require Import NoUninitRefs.
 From Elo Require Import UniqueInits.
+From Elo Require Import UniqueCRs.
 From Elo Require Import ConsistentInits.
 
 (* ------------------------------------------------------------------------- *)
 (* init-cr-exclusivity                                                       *)
 (* ------------------------------------------------------------------------- *)
 
-Definition init_cr_exclusivity (m : mem) (ths : threads) := forall ad tid1 tid2,
+Definition init_cr_exclusivity (ths : threads) := forall ad tid1 tid2,
   (one_init ad ths[tid1] -> no_cr   ad ths[tid2]) /\
   (one_cr   ad ths[tid1] -> no_init ad ths[tid2]).
 
 (* preservation ------------------------------------------------------------ *)
 
-Lemma ice_preservation_none : forall m ths tid t,
+Lemma ice_preservation_none : forall ths tid t,
   forall_threads ths valid_blocks ->
   (* --- *)
-  init_cr_exclusivity m ths ->
+  init_cr_exclusivity ths ->
   ths[tid] --[e_none]--> t ->
-  init_cr_exclusivity m ths[tid <- t].
+  init_cr_exclusivity ths[tid <- t].
 Proof.
   intros * ? Hice ? ad tid1 tid2.
   destruct (Hice ad tid1 tid2) as [? ?].
@@ -32,11 +34,12 @@ Lemma ice_preservation_alloc : forall m ths tid t T,
   forall_threads ths (valid_addresses m) ->
   forall_threads ths valid_blocks ->
   (* --- *)
-  init_cr_exclusivity m ths ->
+  init_cr_exclusivity ths ->
   ths[tid] --[e_alloc (#m) T]--> t ->
-  init_cr_exclusivity (m +++ (None, T, false)) ths[tid <- t].
+  init_cr_exclusivity ths[tid <- t].
 Proof.
-  intros * Hvad ? Hice ? ad tid1 tid2.
+  intros until 2.
+  intros Hice ? ad tid1 tid2.
   destruct (Hice ad tid1 tid2) as [? ?].
   assert (forall tid, no_cr (#m) ths[tid]) by eauto using nocr_from_vad.
   split; intros; repeat omicron; auto; destruct (nat_eq_dec ad (#m)); subst;
@@ -45,7 +48,7 @@ Proof.
   exfalso; eauto using onecr_inheritance_alloc, nocr_onecr_contradiction.
 Qed.
 
-Theorem insert_then_noinit : forall m ths tid t ad te,
+Theorem oneinit_from_insert : forall m ths tid t ad te,
   forall_threads ths (valid_addresses m) ->
   forall_threads ths (consistent_inits m) ->
   unique_initializers m ths ->
@@ -61,18 +64,200 @@ Proof.
   exfalso. eauto using noinit_insert_contradiction.
 Qed.
 
+Theorem onecr_from_rel : forall m ths tid t ad,
+  unique_critical_regions m ths ->
+  (* --- *)
+  ths[tid] --[e_rel ad]--> t ->
+  one_cr ad ths[tid].
+Proof.
+  intros * Hucr **. specialize (Hucr ad) as [Hfalse Htrue].
+  destruct (m[ad].X) eqn:?.
+  - specialize (Htrue eq_refl) as [tid' [? ?]]; clear Hfalse.
+    destruct (nat_eq_dec tid' tid); subst; trivial.
+    exfalso. eauto using nocr_rel_contradiction.
+  - specialize (Hfalse eq_refl); clear Htrue.
+    exfalso. eauto using nocr_rel_contradiction.
+Qed.
+
 Lemma ice_preservation_insert : forall m ths tid t ad te,
+  forall_threads ths (valid_addresses m) ->
+  forall_threads ths valid_blocks ->
+  forall_threads ths (consistent_inits m) ->
+  unique_initializers m ths ->
+  unique_critical_regions m ths ->
+  (* --- *)
+  init_cr_exclusivity ths ->
+  ths[tid] --[e_insert ad te]--> t ->
+  init_cr_exclusivity ths[tid <- t].
+Proof.
+  intros until 5. rename ad into ad'.
+  intros Hice ? ad tid1 tid2.
+  destruct (Hice ad tid1 tid2) as [? ?].
+  split; intros; repeat omicron; auto; destruct (nat_eq_dec ad' ad); subst;
+  eauto using nocr_preservation_insert, oneinit_inheritance_insert;
+  eauto using noinit_preservation_insert, onecr_inheritance_insert;
+  exfalso.
+  - assert (one_init ad ths[tid2]) by eauto using oneinit_from_insert.
+    assert (no_init ad t) by eauto using oneinit_to_noinit.
+    eauto using noinit_oneinit_contradiction.
+  - assert (one_init ad ths[tid1]) by eauto using oneinit_from_insert.
+    assert (no_init ad t) by eauto using oneinit_to_noinit.
+    eauto using noinit_oneinit_contradiction.
+  - assert (one_cr ad ths[tid2]) by eauto using onecr_inheritance_insert.
+    aspecialize. eauto using noinit_insert_contradiction.
+  - aspecialize. eauto using noinit_insert_contradiction.
+Qed.
+
+Lemma ice_preservation_read : forall m ths tid t ad te,
+  forall_memory m no_inits ->
+  forall_memory m no_crs ->
   forall_threads ths valid_blocks ->
   (* --- *)
-  init_cr_exclusivity m ths ->
-  ths[tid] --[e_insert ad te]--> t ->
-  init_cr_exclusivity m ths[tid <- t].
+  m[ad].t = Some te ->
+  init_cr_exclusivity ths ->
+  ths[tid] --[e_read ad te]--> t ->
+  init_cr_exclusivity ths[tid <- t].
+Proof.
+  intros * Hnoinits Hnocrs ?. rename ad into ad'.
+  intros Had' Hice ? ad tid1 tid2.
+  specialize (Hnoinits ad' _ Had').
+  specialize (Hnocrs ad' _ Had').
+  destruct (Hice ad tid1 tid2) as [? ?].
+  split; intros; repeat omicron; auto;
+  eauto using nocr_preservation_read, oneinit_inheritance_read;
+  eauto using noinit_preservation_read, onecr_inheritance_read.
+Qed.
+
+Lemma ice_preservation_write : forall ths tid t ad te,
+  forall_threads ths valid_blocks ->
+  (* --- *)
+  init_cr_exclusivity ths ->
+  ths[tid] --[e_write ad te]--> t ->
+  init_cr_exclusivity ths[tid <- t].
 Proof.
   intros until 1. rename ad into ad'.
   intros Hice ? ad tid1 tid2.
   destruct (Hice ad tid1 tid2) as [? ?].
   split; intros; repeat omicron; auto; destruct (nat_eq_dec ad' ad); subst;
-  eauto using nocr_preservation_insert, oneinit_inheritance_insert;
-  eauto using noinit_preservation_insert, onecr_inheritance_insert.
-  -
+  eauto using nocr_preservation_write, oneinit_inheritance_write;
+  eauto using noinit_preservation_write, onecr_inheritance_write.
 Qed.
+
+Lemma oneinit_then_uninitialized : forall ad m t,
+  consistent_inits m t ->
+  one_init ad t ->
+  m[ad].t = None.
+Proof.
+  intros. induction t; invc_ci; invc_oneinit; auto.
+Qed.
+
+Lemma noref_from_oneinit : forall ad m ths tid,
+  forall_threads ths (consistent_inits m) ->
+  no_uninitialized_references m ths ->
+  (* --- *)
+  one_init ad ths[tid] ->
+  forall_threads ths (no_ref ad).
+Proof.
+  intros * ? Hnur ?.
+  assert (Hnone : m[ad].t = None) by eauto using oneinit_then_uninitialized.
+  specialize (Hnur ad Hnone) as [_ ?]. assumption.
+Qed.
+
+Lemma ice_preservation_acq : forall m ths tid t ad te,
+  forall_memory m no_inits ->
+  forall_memory m no_crs ->
+  forall_threads ths valid_blocks ->
+  forall_threads ths (consistent_inits m) ->
+  no_uninitialized_references m ths ->
+  unique_initializers m ths ->
+  (* --- *)
+  m[ad].t = Some te ->
+  init_cr_exclusivity ths ->
+  ths[tid] --[e_acq ad te]--> t ->
+  init_cr_exclusivity ths[tid <- t].
+Proof.
+  intros * Hnoinits Hnocrs ? ? Hnur Hui. rename ad into ad'.
+  intros Hsome Hice ? ad tid1 tid2.
+  assert (m[ad'].t <> None) by auto.
+  assert (Had : ad' < #m) by (lt_eq_gt ad' (#m); sigma; upsilon; eauto).
+  specialize (Hnoinits ad' _ Hsome).
+  specialize (Hnocrs ad' _ Hsome).
+  specialize (Hice ad tid1 tid2) as [? ?].
+  split; intros; repeat omicron; auto; destruct (nat_eq_dec ad' ad); subst;
+  eauto using nocr_preservation_acq, oneinit_inheritance_acq;
+  eauto using noinit_preservation_acq, onecr_inheritance_acq.
+  - exfalso. eapply noref_acq_contradiction; eauto.
+    assert (one_init ad ths[tid2]) by eauto using oneinit_inheritance_acq.
+    eapply noref_from_oneinit; eauto.
+  - exfalso. eapply noref_acq_contradiction; eauto.
+    eapply noref_from_oneinit; eauto.
+  - specialize (Hui ad Had) as [Hnone _]. aspecialize.
+    eauto using noinit_preservation_acq.
+  - specialize (Hui ad Had) as [Hnone _]. aspecialize.
+    eauto.
+Qed.
+
+Lemma ice_preservation_rel : forall m ths tid t ad,
+  unique_critical_regions m ths ->
+  (* --- *)
+  init_cr_exclusivity ths ->
+  ths[tid] --[e_rel ad]--> t ->
+  init_cr_exclusivity ths[tid <- t].
+Proof.
+  intros until 1. rename ad into ad'.
+  intros Hice ? ad tid1 tid2.
+  destruct (Hice ad tid1 tid2) as [? ?].
+  split; intros; repeat omicron; auto;  destruct (nat_eq_dec ad' ad); subst;
+  eauto using nocr_preservation_rel, oneinit_inheritance_rel;
+  eauto using noinit_preservation_rel, onecr_inheritance_rel;
+  eauto using onecr_from_rel;
+  exfalso.
+  - eauto using onecr_from_rel, noinit_preservation_rel,
+      noinit_oneinit_contradiction.
+  - eauto using onecr_from_rel, nocr_onecr_contradiction.
+  - eauto using onecr_from_rel, onecr_to_nocr, nocr_onecr_contradiction.
+Qed.
+
+Lemma ice_preservation_spawn : forall ths tid t te,
+  forall_threads ths valid_blocks ->
+  (* --- *)
+  init_cr_exclusivity ths ->
+  ths[tid] --[e_spawn (#ths) te]--> t ->
+  init_cr_exclusivity (ths[tid <- t] +++ te).
+Proof.
+  intros until 1.
+  intros Hice ? ad tid1 tid2.
+  destruct (Hice ad tid1 tid2) as [? ?].
+  assert (no_init ad te) by eauto using noinit_spawn_term.
+  assert (no_cr ad te) by eauto using nocr_spawn_term.
+  split; intros; repeat omicron; auto; eauto using no_cr;
+  eauto using nocr_preservation_spawn, oneinit_inheritance_spawn;
+  eauto using noinit_preservation_spawn, onecr_inheritance_spawn;
+  exfalso; eauto using noinit_oneinit_contradiction, nocr_onecr_contradiction.
+Qed.
+
+Theorem ice_preservation : forall m1 m2 ths1 ths2 tid e,
+  forall_memory m1 no_inits ->
+  forall_memory m1 no_crs ->
+  forall_threads ths1 (valid_addresses m1) ->
+  forall_threads ths1 valid_blocks ->
+  forall_threads ths1 (consistent_inits m1) ->
+  no_uninitialized_references m1 ths1 ->
+  unique_initializers m1 ths1 ->
+  unique_critical_regions m1 ths1 ->
+  (* --- *)
+  init_cr_exclusivity ths1 ->
+  m1 / ths1 ~~[tid, e]~~> m2 / ths2 ->
+  init_cr_exclusivity ths2.
+Proof.
+  intros. invc_cstep; try invc_mstep.
+  - eauto using ice_preservation_none.
+  - eauto using ice_preservation_alloc.
+  - eauto using ice_preservation_insert.
+  - eauto using ice_preservation_read.
+  - eauto using ice_preservation_write.
+  - eauto using ice_preservation_acq.
+  - eauto using ice_preservation_rel.
+  - eauto using ice_preservation_spawn.
+Qed.
+
