Boundaries1.v
@@ -1,6 +1,6 @@
 From Elo Require Import Core.
 
-From Elo Require Import Properties.
+From Elo Require Import NoWRef.
 
 (* ------------------------------------------------------------------------- *)
 (* safe-newx                                                                 *)
