PointerTypes.v
@@ -1,6 +1,8 @@
 From Elo Require Import Core.
 
-From Elo Require Import Properties.
+From Elo Require Import Properties1.
+
+From Elo Require Import ConsistentRefs.
 
 From Elo Require Import AccessCore.
 
