Promise.v
@@ -1,6 +1,11 @@
 From Elo Require Import Core.
-From Elo Require Import Properties.
 
+From Elo Require Import Properties1.
+
+From Elo Require Import NoUninitRefs.
+From Elo Require Import ConsistentRefs.
+
+From Elo Require Import NoWRef.
 From Elo Require Import AccessCore.
 From Elo Require Import PointerTypes.
 From Elo Require Import Inheritance.
